ironfleet/src/Dafny/Distributed/Impl/Raft/CTypes.i.dfy
@@ -1,19 +1,55 @@
-include "../../Services/Raft/AppStateMachine.s.dfy"
-include "../../Common/Framework/Environment.s.dfy"
 include "../../Common/Native/Io.s.dfy"
+include "../../Common/Native/NativeTypes.s.dfy"
+include "../../Protocol/Raft/Types.i.dfy"
 include "AppInterface.i.dfy"
 
 module Raft__CTypes_i {
 
-import opened Raft__AppInterface_i
-import opened AppStateMachine_s
-import opened Environment_s
 import opened Native__Io_s
+import opened Native__NativeTypes_s
+import opened Raft__AppInterface_i
+import opened Raft__Types_i
 
-datatype CLogEntry = CLogEntry(term:uint64, index:uint64, req:CAppRequest, is_commited:bool)
+datatype CClockReading = CClockReading(t:uint64)
 
-predicate CLogEntryValid(entry:CLogEntry) {
-  && entry.term > 0 && entry.index > 0
+function AbstractifyCClockReadingToClockReading(cclock:CClockReading) : ClockReading
+{
+  ClockReading(cclock.t as int)
+}
+
+datatype CLogEntry = CLogEntry(term:uint64, index:uint64, req:CAppRequest, is_commited:uint64)
+
+predicate method ValidLogEntry(entry:CLogEntry) {
+  && 0 < entry.term <= 0xFFFF_FFFF_FFFF_FFFF
+  && 0 < entry.index <= 0xFFFF_FFFF_FFFF_FFFF
+  && (entry.is_commited == 0 || entry.is_commited == 1)
+  && CAppRequestMarshallable(entry.req)
+}
+
+function method LogEntrySeqSizeLimit() : int { 100 }
+
+predicate method ValidLogEntrySeq(entries:seq<CLogEntry>) {
+  && (forall entry :: entry in entries ==> ValidLogEntry(entry))
+  && |entries| <= LogEntrySeqSizeLimit()
+}
+
+predicate CLogEntryIsAbstractable(entry:CLogEntry) {
+  true
+}
+
+predicate CLogEntrySeqIsAbstractable(log_entries:seq<CLogEntry>) {
+  true
+}
+
+function AbstractifyCLogEntryToRaftLogEntry(entry:CLogEntry) : LogEntry
+{
+  LogEntry(entry.term as int, entry.index as int, AbstractifyCAppRequestToAppRequest(entry.req), entry.is_commited == 1)
+}
+
+function AbstractifyCLogEntrySeqToRaftLogEntrySeq(entries:seq<CLogEntry>) : seq<LogEntry>
+{
+  if |entries| == 0 then []
+  else [AbstractifyCLogEntryToRaftLogEntry(entries[0])] + AbstractifyCLogEntrySeqToRaftLogEntrySeq(entries[1..])
 }
 
 }
