ironfleet/src/Dafny/Distributed/Impl/Raft/Config.i.dfy
@@ -3,7 +3,9 @@ include "../../Common/Collections/Sets.i.dfy"
 include "../../Common/Collections/Seqs.i.dfy"
 include "../../Common/Collections/Maps2.s.dfy"
 include "../../Common/Native/NativeTypes.s.dfy"
+include "../Common/SeqIsUniqueDef.i.dfy"
 include "../Common/UpperBound.i.dfy"
+include "../Common/NetClient.i.dfy"
 include "../../Protocol/Raft/Config.i.dfy"
 
 module Raft__ConfigState_i {
@@ -14,6 +16,8 @@ import opened Native__NativeTypes_s
 import opened Collections__Sets_i
 import opened Collections__Seqs_i
 import opened Collections__Maps2_s
+import opened Common__SeqIsUniqueDef_i
+import opened Common__NetClient_i
 import opened Raft__Config_i
 
 datatype ParamState = ParamState(
@@ -22,6 +26,20 @@ datatype ParamState = ParamState(
   heartbeat_timeout:uint64,
   max_integer_value:uint64
 )
+
+predicate ParamStateIsValid(params:ParamState)
+{
+  && params.min_election_timeout <= params.max_election_timeout
+  && params.heartbeat_timeout > 0
+  && params.max_integer_value > 0
+}
+
+method GenerateElectionTimeout(params:ParamState) returns (t:uint64)
+  requires ParamStateIsValid(params)
+  ensures params.min_election_timeout <= t <= params.max_election_timeout
+{
+  t := params.min_election_timeout;
+}
 
 function AbstractifyParamStateToRaftParam(params:ParamState) : RaftParam
 {
@@ -48,6 +66,21 @@ datatype ConfigState = ConfigState(
   server_eps:seq<EndPoint>,
   params:ParamState
 )
+
+predicate ConfigStateIsAbstractable(config:ConfigState)
+{
+  && (forall e :: e in config.server_eps ==> EndPointIsValidPublicKey(e))
+  && SeqIsUnique(config.server_eps)
+}
+
+predicate ConfigStateIsValid(config:ConfigState)
+  ensures ConfigStateIsValid(config) ==> SeqIsUnique(config.server_eps)
+{
+  && 0 < |config.server_eps| < 0xffff_ffff_ffff_ffff
+  && ConfigStateIsAbstractable(config)
+  && ParamStateIsValid(config.params)
+  && RaftMinQuorumSize(AbstractifyConfigStateToRaftConfig(config)) <= |config.server_eps|
+}
 
 function AbstractifyConfigStateToRaftConfig(config:ConfigState) : RaftConfig
 {
@@ -78,6 +111,12 @@ method InitServerConfigState(my_ep:EndPoint, eps:seq<EndPoint>) returns (sc:Serv
   var params := StaticParams(); 
   var global_config := ConfigState(eps, params);
   sc := ServerConfigState(my_ep, global_config);
+}
+
+function method RaftEndPointIsValid(endPoint:EndPoint, config:ConfigState) : bool
+  requires ConfigStateIsValid(config)
+{
+  EndPointIsValidPublicKey(endPoint)
 }
 
 }
