ironfleet/src/Dafny/Distributed/Impl/Raft/PacketParsing.i.dfy
@@ -1,24 +1,34 @@
-include "../../Common/Collections/Maps.i.dfy"
+include "../../../Libraries/Math/mul.i.dfy"
+include "../../Common/Framework/Environment.s.dfy"
+include "../../Common/Native/Io.s.dfy"
+include "../../Common/Native/NativeTypes.s.dfy"
+// include "../../Common/Collections/Maps.i.dfy"
 include "../../Protocol/Raft/Types.i.dfy"
+include "../../Services/Raft/AppStateMachine.s.dfy"
 include "../Common/GenericMarshalling.i.dfy"
+include "../Common/NetClient.i.dfy"
+include "../Common/NodeIdentity.i.dfy"
+include "AppInterface.i.dfy"
+include "CMessage.i.dfy"
 include "CTypes.i.dfy"
+
 
 module Raft__PacketParsing_i {
 
+import opened Math__mul_i
+import opened Environment_s
 import opened Native__Io_s
 import opened Native__NativeTypes_s
-import opened Collections__Maps_i
-import opened Raft__AppInterface_i
+// import opened Collections__Maps_i
 import opened Raft__Types_i
-import opened Raft__CTypes_i
 import opened Common__GenericMarshalling_i
-import opened Common__NodeIdentity_i
 import opened Common__NetClient_i
-import opened Common__Util_i
+import opened Common__NodeIdentity_i
+// import opened Common__Util_i
 import opened AppStateMachine_s
-import opened Environment_s
-import opened Math__mul_i
-import opened Math__mul_nonlinear_i
+import opened Raft__AppInterface_i
+import opened Raft__CMessage_i
+import opened Raft__CTypes_i
 
 ////////////////////////////////////////////////////////////////////
 //    Grammars for the Rafy types
@@ -54,29 +64,34 @@ predicate CMessageIs64Bit(msg:CMessage)
   true
 }
 
+predicate CLogEntrySeqIs64Bit(entries:seq<CLogEntry>)
+{
+  true
+}
 
 ////////////////////////////////////////////////////////////////////
 //    Parsing
 ////////////////////////////////////////////////////////////////////
 function method parse_EndPoint(val:V) : EndPoint
   requires ValInGrammar(val, EndPoint_grammar())
-  ensures  EndPointIsAbstractable(parse_EndPoint(val))
+  ensures EndPointIsAbstractable(parse_EndPoint(val))
 {
   EndPoint(val.b)
 }
 
-function method parse_CLogEntry(val:V) : CLogEntry
+function method parse_LogEntry(val:V) : CLogEntry
   requires ValInGrammar(val, CLogEntry_grammar())
-  ensures  CLogEntryIsAbstractable(parse_CLogEntry(val))
+  ensures CLogEntryIsAbstractable(parse_LogEntry(val))
 {
+  assert ValInGrammar(val, CLogEntry_grammar());
   CLogEntry(val.t[0].u, val.t[1].u, val.t[2].b, val.t[3].u)
 }
 
 function method parse_Message_RequestVote(val:V) : CMessage
   requires ValInGrammar(val, CMessage_RequestVote_grammar())
-  ensures CMesssageIsAbstractable(parse_Message_RequestVote(val))
-  ensures  ValidVal(val) ==> CMessageIs64Bit(parse_Message_RequestVote(val))
+  ensures CMessageIsAbstractable(parse_Message_RequestVote(val))
 {
+  assert ValInGrammar(val, CMessage_RequestVote_grammar());
   CMessage_RequestVote(
     val.t[0].u,
     parse_EndPoint(val.t[1]),
@@ -87,52 +102,55 @@ function method parse_Message_RequestVote(val:V) : CMessage
 
 function method parse_Message_RequestVoteReply(val:V) : CMessage
   requires ValInGrammar(val, CMessage_RequestVoteReply_grammar())
-  ensures CMesssageIsAbstractable(parse_Message_RequestVoteReply(val))
+  ensures CMessageIsAbstractable(parse_Message_RequestVoteReply(val))
   ensures  ValidVal(val) ==> CMessageIs64Bit(parse_Message_RequestVoteReply(val))
 {
+  assert ValInGrammar(val, CMessage_RequestVoteReply_grammar());
   CMessage_RequestVoteReply(
     val.t[0].u,
     val.t[1].u
   )
 }
 
-function parse_CLogEntrySeq(val:V) : seq<CLogEntry>
-  requires ValInGrammar(val, CLogEntrySeq())
-  ensures  |parse_CLogEntrySeq(val)| == |val.a|
-  ensures  forall i :: 0 <= i < |parse_CLogEntrySeq(val)| ==> parse_CLogEntrySeq(val)[i] == parse_CLogEntry(val.a[i])
-  ensures  CRequestBatchIsAbstractable(parse_CLogEntrySeq(val))
-  ensures  ValidVal(val) ==> CRequestBatchIs64Bit(parse_CLogEntrySeq(val))
+function method parse_LogEntrySeq(val:V) : seq<CLogEntry>
+  requires ValInGrammar(val, CLogEntrySeq_grammar())
+  ensures  |parse_LogEntrySeq(val)| == |val.a|
+  ensures  forall i :: 0 <= i < |parse_LogEntrySeq(val)| ==> parse_LogEntrySeq(val)[i] == parse_LogEntry(val.a[i])
+  ensures  CLogEntrySeqIsAbstractable(parse_LogEntrySeq(val))
+  ensures  ValidVal(val) ==> CLogEntrySeqIs64Bit(parse_LogEntrySeq(val))
   decreases |val.a|
 {
   if |val.a| == 0 then
     []
   else 
-    var req := parse_CLogEntry(val.a[0]);
+    var req := parse_LogEntry(val.a[0]);
     var restVal:V := VArray(val.a[1..]);
-    var rest := parse_CLogEntrySeq(restVal);
+    var rest := parse_LogEntrySeq(restVal);
     [req] + rest
 }
 
 function method parse_Message_AppendEntries(val:V) : CMessage
   requires ValInGrammar(val, CMessage_AppendEntries_grammar())
-  ensures CMesssageIsAbstractable(parse_Message_AppendEntries(val))
+  ensures CMessageIsAbstractable(parse_Message_AppendEntries(val))
   ensures  ValidVal(val) ==> CMessageIs64Bit(parse_Message_AppendEntries(val))
 {
+  assert ValInGrammar(val, CMessage_AppendEntries_grammar());
   CMessage_AppendEntries(
     val.t[0].u,
     parse_EndPoint(val.t[1]),
     val.t[2].u,
     val.t[3].u,
-    parse_CLogEntrySeq(val.t[4]),
+    parse_LogEntrySeq(val.t[4]),
     val.t[5].u
   )
 }
 
 function method parse_Message_AppendEntriesReply(val:V) : CMessage
   requires ValInGrammar(val, CMessage_AppendEntriesReply_grammar())
-  ensures CMesssageIsAbstractable(parse_Message_AppendEntriesReply(val))
+  ensures CMessageIsAbstractable(parse_Message_AppendEntriesReply(val))
   ensures  ValidVal(val) ==> CMessageIs64Bit(parse_Message_AppendEntriesReply(val))
 {
+  assert ValInGrammar(val, CMessage_AppendEntriesReply_grammar());
   CMessage_AppendEntriesReply(
     val.t[0].u,
     val.t[1].u,
@@ -140,10 +158,28 @@ function method parse_Message_AppendEntriesReply(val:V) : CMessage
   )
 }
 
+function parse_Message(val:V) : CMessage
+  requires ValInGrammar(val, CMessage_grammar())
+  ensures  CMessageIsAbstractable(parse_Message(val))
+  ensures  ValidVal(val) ==> CMessageIs64Bit(parse_Message(val))
+{
+  if val.c == 0 then
+    parse_Message_RequestVote(val.val)
+  else if val.c == 1 then
+    parse_Message_RequestVoteReply(val.val)
+  else if val.c == 2 then
+    parse_Message_AppendEntries(val.val)
+  else if val.c == 3 then
+    parse_Message_AppendEntriesReply(val.val)
+  else
+    assert false;
+    parse_Message_RequestVote(val.val)
+}
+
 method Parse_Message(val:V) returns (msg:CMessage)
 	requires ValInGrammar(val, CMessage_grammar())
 	requires ValidVal(val)
-	// ensures	 msg == parse_Message(val)
+	ensures	 msg == parse_Message(val)
 	ensures	 !msg.CMessage_Invalid?
 	ensures	 CMessageIsAbstractable(msg)
 	ensures	 CMessageIs64Bit(msg)
@@ -199,14 +235,14 @@ method RaftDemarshallDataMethod(data:array<byte>, msg_grammar:G) returns (msg:CM
 ////////////////////////////////////////////////////////////////////
 //    Can a value be marshalled?
 ////////////////////////////////////////////////////////////////////
-function Marshallable(msg:CMessage) : bool
+function Marshallable(c:CMessage) : bool
 {
   // TODO: this is a hack
-  && (!msg.CMessage_Invalid?)
-  && (msg.CMessage_RequestVote? ==> true)
-  && (msg.CMessage_RequestVoteReply? ==> true)
-  && (msg.CMessage_AppendEntries? ==> true)
-  && (msg.CMessage_AppendEntriesReply? ==> true)
+  && (!c.CMessage_Invalid?)
+  && (c.CMessage_RequestVote? ==> EndPointIsValidPublicKey(c.candidate_ep))
+  && (c.CMessage_RequestVoteReply? ==> true)
+  && (c.CMessage_AppendEntries? ==> ValidAppendEntries(c) && EndPointIsValidPublicKey(c.leader_ep))
+  && (c.CMessage_AppendEntriesReply? ==> true)
 }
 
 function CMessageIsValid(msg:CMessage) : bool
@@ -219,7 +255,397 @@ predicate CPacketsIsMarshallable(cps:set<CPacket>)
   forall cp :: cp in cps ==> Marshallable(cp.msg)
 }
 
-// TODO & DOING: finish this about determining if valid and DetermineIfMessageMarshallable
+method DetermineIfMessageMarshallable(msg:CMessage) returns (b:bool)
+  requires CMessageIsAbstractable(msg)
+  requires CMessageIs64Bit(msg)
+  ensures  b == Marshallable(msg)
+{
+  if msg.CMessage_Invalid? {
+    b := false;
+  }
+  else if msg.CMessage_RequestVote? {
+    b := EndPointIsValidPublicKey(msg.candidate_ep);
+  }
+  else if msg.CMessage_RequestVoteReply? {
+    b := true;
+  }
+  else if msg.CMessage_AppendEntries? {
+    b := ValidAppendEntries(msg) && EndPointIsValidPublicKey(msg.leader_ep);
+  }
+  else if msg.CMessage_AppendEntriesReply? {
+    b := true;
+  }
+  else {
+    assert false;
+  }
+}
 
+////////////////////////////////////////////////////////////////////
+//    Marshalling 
+////////////////////////////////////////////////////////////////////
+method MarshallEndPoint(c:EndPoint) returns (val:V)
+  requires EndPointIsValidPublicKey(c)
+  ensures  ValInGrammar(val, EndPoint_grammar())
+  ensures  ValidVal(val)
+  ensures  parse_EndPoint(val) == c
+{
+  val := VByteArray(c.public_key);
+}
+
+method MarshallLogEntry(c:CLogEntry) returns (val:V)
+  requires ValidLogEntry(c)
+  ensures ValInGrammar(val, CLogEntry_grammar())
+  ensures ValidVal(val)
+  ensures parse_LogEntry(val) == c
+{
+  var marshalled_app_req := MarshallCAppRequest(c.req);
+  val := VTuple([VUint64(c.term), VUint64(c.index), marshalled_app_req, VUint64(c.is_commited)]);
+  assert ValInGrammar(val, CLogEntry_grammar());
+}
+
+method MarshallLogEntrySeq(c:seq<CLogEntry>) returns (val:V)
+  requires ValidLogEntrySeq(c)
+  ensures ValInGrammar(val, CLogEntrySeq_grammar())
+  ensures ValidVal(val)
+  ensures parse_LogEntrySeq(val) == c
+{
+  var reqs := new V[|c| as uint64];
+
+  var i:uint64 := 0;
+  while i < |c| as uint64
+    invariant 0 <= i as int <= |c|
+    invariant forall j :: 0 <= j < i ==> ValInGrammar(reqs[j], CLogEntry_grammar())
+    invariant forall j :: 0 <= j < i ==> ValidVal(reqs[j])
+    invariant forall j :: 0 <= j < i ==> parse_LogEntry(reqs[j]) == c[j]
+  {
+    var single := MarshallLogEntry(c[i]);
+    assert ValInGrammar(single, CLogEntry_grammar());
+    reqs[i] := single;
+    i := i + 1;
+  }
+
+  val := VArray(reqs[..]);
+}
+
+method MarshallMessage_RequestVote(c:CMessage) returns (val:V)
+  requires c.CMessage_RequestVote?
+  requires ValidRequestVote(c)
+  requires Marshallable(c)
+  ensures  ValInGrammar(val, CMessage_RequestVote_grammar())
+  ensures  ValidVal(val)
+  ensures  parse_Message_RequestVote(val) == c
+{
+  var marshalled_ep := MarshallEndPoint(c.candidate_ep);
+  val := VTuple([VUint64(c.term), marshalled_ep, VUint64(c.last_log_index), VUint64(c.last_log_term)]);
+  assert ValInGrammar(val, CMessage_RequestVote_grammar());
+}
+
+method MarshallMessage_RequestVoteReply(c:CMessage) returns (val:V)
+  requires c.CMessage_RequestVoteReply?
+  requires Marshallable(c)
+  ensures  ValInGrammar(val, CMessage_RequestVoteReply_grammar())
+  ensures  ValidVal(val)
+  ensures  parse_Message_RequestVoteReply(val) == c
+{
+  val := VTuple([VUint64(c.term), VUint64(c.vote_granted)]);
+  assert ValInGrammar(val, CMessage_RequestVoteReply_grammar());
+}
+
+method MarshallMessage_AppendEntries(c:CMessage) returns (val:V)
+  requires c.CMessage_AppendEntries?
+  requires ValidAppendEntries(c)
+  requires Marshallable(c)
+  ensures  ValInGrammar(val, CMessage_AppendEntries_grammar())
+  ensures  ValidVal(val)
+  ensures  parse_Message_AppendEntries(val) == c
+{
+  var marshalled_ep := MarshallEndPoint(c.leader_ep);
+  var marshalled_entries := MarshallLogEntrySeq(c.entries);
+  val := VTuple([
+    VUint64(c.term), 
+    marshalled_ep, 
+    VUint64(c.prev_log_index), 
+    VUint64(c.prev_log_term), 
+    marshalled_entries, 
+    VUint64(c.leader_commit)
+  ]);
+  assert ValInGrammar(val, CMessage_AppendEntries_grammar());
+}
+
+method MarshallMessage_AppendEntriesReply(c:CMessage) returns (val:V)
+  requires c.CMessage_AppendEntriesReply?
+  requires Marshallable(c)
+  ensures  ValInGrammar(val, CMessage_AppendEntriesReply_grammar())
+  ensures  ValidVal(val)
+  ensures  parse_Message_AppendEntriesReply(val) == c
+{
+  val := VTuple([VUint64(c.term), VUint64(c.success), VUint64(c.match_index)]);
+  assert ValInGrammar(val, CMessage_AppendEntriesReply_grammar());
+}
+
+method MarshallMessage(c:CMessage) returns (val:V)
+  requires Marshallable(c)
+  ensures  ValInGrammar(val, CMessage_grammar())
+  ensures  ValidVal(val)
+  ensures  parse_Message(val) == c
+{
+  assert !c.CMessage_Invalid?;
+  if c.CMessage_RequestVote? {
+    assert EndPointIsValidPublicKey(c.candidate_ep);
+    var msg := MarshallMessage_RequestVote(c);
+    val := VCase(0, msg);
+  } else if c.CMessage_RequestVoteReply? {
+    var msg := MarshallMessage_RequestVoteReply(c);
+    val := VCase(1, msg);
+  } else if c.CMessage_AppendEntries? {
+    var msg := MarshallMessage_AppendEntries(c);
+    val := VCase(2, msg);
+  } else if c.CMessage_AppendEntriesReply? {
+    var msg := MarshallMessage_AppendEntriesReply(c);
+    val := VCase(3, msg);
+  } else {
+    assert false;
+  }
+}
+
+////////////////////////////////////////////////////////////////////////
+// These functions need to be here, rather than CMessageRefinements.i.dfy,
+// since they depend on RaftDemarshallData
+////////////////////////////////////////////////////////////////////////
+
+predicate NetPacketIsAbstractable(net:NetPacket)
+{
+  && EndPointIsValidPublicKey(net.src)
+  && EndPointIsValidPublicKey(net.dst)
+}
+
+function AbstractifyBufferToRaftPacket(src:EndPoint, dst:EndPoint, data:seq<byte>) : RaftPacket
+  requires EndPointIsValidPublicKey(src)
+  requires EndPointIsValidPublicKey(dst)
+{
+  LPacket(AbstractifyEndPointToNodeIdentity(dst),
+          AbstractifyEndPointToNodeIdentity(src),
+          AbstractifyCMessageToRaftMessage(RaftDemarshallData(data)))
+}
+
+function AbstractifyNetPacketToRaftPacket(net:NetPacket) : RaftPacket
+  requires NetPacketIsAbstractable(net)
+{
+  AbstractifyBufferToRaftPacket(net.src, net.dst, net.msg)
+}
+
+lemma lemma_CMessageGrammarValid()
+  ensures ValidGrammar(CMessage_grammar())
+{
+  var g := CMessage_grammar();
+  assert |g.cases| < 0x1_0000_0000_0000_0000;
+  assert ValidGrammar(CMessage_RequestVote_grammar());
+  assert ValidGrammar(CMessage_RequestVoteReply_grammar());
+  assert ValidGrammar(CMessage_AppendEntries_grammar());
+  assert ValidGrammar(CMessage_AppendEntriesReply_grammar());
+}
+
+predicate CBroadcastIsValid(broadcast:CBroadcast) 
+{
+  && CBroadcastIsAbstractable(broadcast)
+  && (broadcast.CBroadcast? ==>
+      && Marshallable(broadcast.msg)
+      && 0 <= |broadcast.dsts| < 0xFFFF_FFFF_FFFF_FFFF)
+}
+
+predicate BufferRefinementAgreesWithMessageRefinement(msg:CMessage, marshalled:seq<byte>)
+  requires CMessageIsAbstractable(msg)
+  requires CMessageIsAbstractable(msg)
+{
+  forall src, dst :: (EndPointIsValidPublicKey(src) && EndPointIsValidPublicKey(dst)) ==>
+
+            (AbstractifyBufferToRaftPacket(src, dst, marshalled)
+            == LPacket(AbstractifyEndPointToNodeIdentity(dst), AbstractifyEndPointToNodeIdentity(src), AbstractifyCMessageToRaftMessage(msg)))
+}
+
+
+lemma lemma_CLogEntryBound(c:CLogEntry, val:V)
+  requires c.CLogEntry?
+  requires ValInGrammar(val, CLogEntry_grammar())
+  requires ValidLogEntry(c)
+  requires parse_LogEntry(val) == c
+  ensures SizeOfV(val) <= 32 + MaxAppRequestSize()
+{
+  assert ValInGrammar(val, CLogEntry_grammar());
+  lemma_VSizeSeqSum4(val);
+  assert SizeOfV(val.t[0]) == 8;
+  assert SizeOfV(val.t[1]) == 8; 
+  assert SizeOfV(val.t[2]) <= 8 + MaxAppRequestSize();
+  assert SizeOfV(val.t[3]) == 8;
+  assert SizeOfV(val) <= 32 + MaxAppRequestSize();
+}
+
+
+lemma lemma_CLogEntrySeqBound(c:seq<CLogEntry>, val:V)
+  requires ValInGrammar(val, CLogEntrySeq_grammar())
+  requires ValidLogEntrySeq(c)
+  requires parse_LogEntrySeq(val) == c
+  decreases |c|
+  ensures SeqSum(val.a) <= (32 + MaxAppRequestSize())*|val.a|
+{
+  ghost var garray := GArray(CLogEntry_grammar());
+  assert ValInGrammar(val, garray);
+  reveal SeqSum();
+  if |val.a| == 0 {
+    assert SeqSum(val.a) <= (32 + MaxAppRequestSize())*|val.a|;
+  } else {
+    var req := parse_LogEntry(val.a[0]);
+    var restVal:V := VArray(val.a[1..]);
+    var rest := parse_LogEntrySeq(restVal);
+    assert c == [req] + rest;
+    var x := 32 + MaxAppRequestSize();
+    var N := |val.a|;
+    lemma_CLogEntrySeqBound(rest, restVal);
+    assert SeqSum(val.a[1..]) <= x * (N-1);
+    lemma_CLogEntryBound(req, val.a[0]);
+    assert SizeOfV(val.a[0]) <= x;
+    assert SeqSum(val.a) == SizeOfV(val.a[0]) + SeqSum(val.a[1..]);
+    assert |val.a| == |val.a[1..]| + 1;
+    lemma_mul_is_distributive(x, N-1, 1);
+    assert SeqSum(val.a) <= x * N;
+  }
+}
+
+lemma lemma_MarshallableBound(c:CMessage, val:V)
+  requires Marshallable(c)
+  requires ValInGrammar(val, CMessage_grammar())
+  requires ValidVal(val)
+  requires parse_Message(val) == c
+  ensures 0 <= SizeOfV(val) < MaxPacketSize()
+{
+  assert !c.CMessage_Invalid?;
+  if c.CMessage_RequestVote? {
+    assert ValInGrammar(val.val, CMessage_RequestVote_grammar());
+    assert ValInGrammar(val.val.t[0], GUint64()) && SizeOfV(val.val.t[0]) == 8;
+    assert ValInGrammar(val.val.t[1], GByteArray()) && SizeOfV(val.val.t[1]) <= 8 + MaxEndpointSize();
+    assert ValInGrammar(val.val.t[2], GUint64()) && SizeOfV(val.val.t[2]) == 8;
+    assert ValInGrammar(val.val.t[3], GUint64()) && SizeOfV(val.val.t[3]) == 8;
+    assert |val.val.t| == 4;
+    lemma_VSizeSeqSum4(val.val);
+    assert SizeOfV(val) <= 40 + MaxEndpointSize();
+  } else if c.CMessage_RequestVoteReply? {
+    assert ValInGrammar(val.val, CMessage_RequestVoteReply_grammar());
+    assert ValInGrammar(val.val.t[0], GUint64()) && SizeOfV(val.val.t[0]) == 8;
+    assert ValInGrammar(val.val.t[1], GUint64()) && SizeOfV(val.val.t[1]) == 8;
+    assert |val.val.t| == 2;
+    lemma_VSizeSeqSum2(val.val);
+    assert SizeOfV(val) == 24;
+  } else if c.CMessage_AppendEntries? {
+    assert ValInGrammar(val.val, CMessage_AppendEntries_grammar());
+    assert SizeOfV(val.val.t[0]) == 8;
+    assert SizeOfV(val.val.t[1]) <= 8 + MaxEndpointSize();
+    assert SizeOfV(val.val.t[2]) <= 8;
+    assert SizeOfV(val.val.t[3]) == 8;
+    lemma_CLogEntrySeqBound(c.entries, val.val.t[4]);
+    assert SizeOfV(val.val.t[4]) <= 8 + (32 + MaxAppRequestSize())*|val.val.t[4].a|;
+    assert |val.val.t[4].a| <= LogEntrySeqSizeLimit();
+    calc {
+      SizeOfV(val.val.t[4]);
+      8 + SeqSum(val.val.t[4].a);
+      <=
+      8 + (32 + MaxAppRequestSize())*|val.val.t[4].a|;
+      <= { lemma_mul_is_commutative(|val.val.t[4].a|, LogEntrySeqSizeLimit());
+          lemma_mul_is_commutative(|val.val.t[4].a|, 32 + MaxAppRequestSize());
+          lemma_mul_inequality(|val.val.t[4].a|, LogEntrySeqSizeLimit(), 32 + MaxAppRequestSize());
+        }
+      8 + (32 + MaxAppRequestSize())*LogEntrySeqSizeLimit();
+    }
+    assert SizeOfV(val.val.t[4]) <= 8 + (32 + MaxAppRequestSize())*LogEntrySeqSizeLimit();
+    assert SizeOfV(val.val.t[5]) == 8;
+    lemma_VSizeSeqSum6(val.val);
+    calc {
+      SizeOfV(val);
+      8 + SizeOfV(val.val);
+      8 + SizeOfV(val.val.t[0]) + SizeOfV(val.val.t[1]) + SizeOfV(val.val.t[2]) + SizeOfV(val.val.t[3]) + SizeOfV(val.val.t[4]) + SizeOfV(val.val.t[5]);
+      8 + 8 + SizeOfV(val.val.t[1]) + 8 + 8 + SizeOfV(val.val.t[4]) + 8;
+      <=
+      8 + 8 + 8 + MaxEndpointSize() + 8 + 8 + SizeOfV(val.val.t[4]) + 8;
+      <=
+      8 + 8 + 8 + MaxEndpointSize() + 8 + 8 + 8 + (32 + MaxAppRequestSize())*|val.val.t[4].a| + 8;
+      ==
+      56 + MaxEndpointSize() + (32 + MaxAppRequestSize())*|val.val.t[4].a|;
+      <= {
+        lemma_mul_is_commutative(|val.val.t[4].a|, LogEntrySeqSizeLimit());
+        lemma_mul_is_commutative(|val.val.t[4].a|, 32 + MaxAppRequestSize());
+        lemma_mul_inequality(|val.val.t[4].a|, LogEntrySeqSizeLimit(), 32 + MaxAppRequestSize());
+      }
+      56 + MaxEndpointSize() + (32 + MaxAppRequestSize())*LogEntrySeqSizeLimit();
+    }
+    assert SizeOfV(val) <= 56 + MaxEndpointSize() + (32 + MaxAppRequestSize())*|val.val.t[4].a|;
+    assert SizeOfV(val) <= 56 + MaxEndpointSize() + (32 + MaxAppRequestSize())*LogEntrySeqSizeLimit();
+  } else if c.CMessage_AppendEntriesReply? {
+    assert ValInGrammar(val.val, CMessage_AppendEntriesReply_grammar());
+    assert ValInGrammar(val.val.t[0], GUint64()) && SizeOfV(val.val.t[0]) == 8;
+    assert ValInGrammar(val.val.t[1], GUint64()) && SizeOfV(val.val.t[1]) == 8;
+    assert ValInGrammar(val.val.t[2], GUint64()) && SizeOfV(val.val.t[2]) == 8;
+    assert |val.val.t| == 3;
+    lemma_VSizeSeqSum3(val.val);
+    assert SizeOfV(val) == 32;
+  } else {
+    assert false;
+  }
+}
+
+method RaftMarshall(msg:CMessage) returns (data:array<byte>)
+  requires CMessageIsAbstractable(msg)
+  requires Marshallable(msg)
+  ensures fresh(data)
+  ensures NetPacketBound(data[..])
+  ensures Marshallable(RaftDemarshallData(data[..]))
+  ensures BufferRefinementAgreesWithMessageRefinement(msg, data[..])
+{
+  var val := MarshallMessage(msg);
+  lemma_MarshallableBound(msg, val);
+  lemma_CMessageGrammarValid();
+  data := Marshall(val, CMessage_grammar());
+
+  forall src, dst | EndPointIsValidPublicKey(src) && EndPointIsValidPublicKey(dst) 
+    ensures AbstractifyBufferToRaftPacket(src, dst, data[..])
+              == LPacket(AbstractifyEndPointToNodeIdentity(dst), AbstractifyEndPointToNodeIdentity(src), AbstractifyCMessageToRaftMessage(msg));
+  {
+    calc {
+      AbstractifyBufferToRaftPacket(src, dst, data[..]);
+      LPacket(AbstractifyEndPointToNodeIdentity(dst),
+              AbstractifyEndPointToNodeIdentity(src),
+              AbstractifyCMessageToRaftMessage(RaftDemarshallData(data[..])));
+      LPacket(AbstractifyEndPointToNodeIdentity(dst),
+              AbstractifyEndPointToNodeIdentity(src),
+              AbstractifyCMessageToRaftMessage(RaftDemarshallData(data[..])));
+      LPacket(AbstractifyEndPointToNodeIdentity(dst), AbstractifyEndPointToNodeIdentity(src), AbstractifyCMessageToRaftMessage(msg));
+    }
+  }
+}
+
+//////////////////////////////////////////////////////////////////////////////
+// Sendable predicates
+
+predicate CPacketIsSendable(cpacket:CPacket)
+{
+  && CMessageIsValid(cpacket.msg) 
+  && CPacketIsAbstractable(cpacket)
+  && EndPointIsValidPublicKey(cpacket.src)
+}
+
+predicate OutboundPacketsIsValid(out:OutboundPackets)
+{
+  match out
+    case Broadcast(broadcast) => CBroadcastIsValid(broadcast)
+    case OutboundPacket(p) => p.Some? ==> CPacketIsSendable(p.v)
+    case PacketSequence(s) => |s| < 0xFFFF_FFFF_FFFF_FFFF 
+                              && (forall p :: p in s ==> CPacketIsSendable(p))
+}
+
+predicate IosReflectIgnoringUnsendable(ios:seq<LIoOp<EndPoint, seq<byte>>>)
+{
+  && |ios| == 1
+  && ios[0].LIoOpReceive?
+  && (|| !Demarshallable(ios[0].r.msg, CMessage_grammar())
+     || !Marshallable(parse_Message(DemarshallFunc(ios[0].r.msg, CMessage_grammar()))))
+}
 
 }
