ironfleet/src/Dafny/Distributed/Impl/Raft/CBroadcast.i.dfy
@@ -1,0 +1,35 @@
+include "../../Common/Native/Io.s.dfy"
+include "../../Protocol/Raft/Types.i.dfy"
+include "../../Protocol/Raft/Server.i.dfy"
+include "../Common/NetClient.i.dfy"
+include "../Common/NodeIdentity.i.dfy"
+include "Config.i.dfy"
+include "CMessage.i.dfy"
+include "PacketParsing.i.dfy"
+
+module Raft__CBroadcast_i {
+
+import opened Native__Io_s
+import opened Native__NativeTypes_s
+import opened Common__NetClient_i
+import opened Common__NodeIdentity_i
+import opened Raft__Types_i
+import opened Raft__ConfigState_i
+import opened Raft__CMessage_i
+import opened Raft__PacketParsing_i
+import opened Raft__Server_i
+
+// CBroadcast
+method BuildBroadcastToEveryone(config:ConfigState, my_ep:EndPoint, msg:CMessage) returns (broadcast:CBroadcast)
+  requires ConfigStateIsValid(config)
+  requires my_ep in config.server_eps
+  requires CMessageIsAbstractable(msg)
+  requires Marshallable(msg)
+  ensures CBroadcastIsValid(broadcast)
+  ensures OutboundPacketsHasCorrectSrc(Broadcast(broadcast), my_ep)
+  ensures RaftBroadcastToEveryone(AbstractifyConfigStateToRaftConfig(config), my_ep, AbstractifyCMessageToRaftMessage(msg), AbstractifyCBroadcastToRaftPacketSeq(broadcast))
+{
+  broadcast := CBroadcast(my_ep, config.server_eps, msg);
+}
+
+}
