ironfleet/src/Dafny/Distributed/Impl/Raft/NetRaft.i.dfy
@@ -1,0 +1,478 @@
+include "../../Common/Native/Io.s.dfy"
+include "../../Common/Native/NativeTypes.s.dfy"
+include "../../Common/Framework/Environment.s.dfy"
+include "../../Protocol/Raft/Types.i.dfy"
+include "../Common/NetClient.i.dfy"
+include "../Common/NodeIdentity.i.dfy"
+include "../Common/NetClient.i.dfy"
+include "../Common/Util.i.dfy"
+include "CBroadcast.i.dfy"
+include "Config.i.dfy"
+include "CTypes.i.dfy"
+include "CMessage.i.dfy"
+include "PacketParsing.i.dfy"
+
+module Raft__NetRaft_i {
+
+import opened Native__Io_s
+import opened Native__NativeTypes_s
+import opened Environment_s
+import opened Raft__Types_i
+import opened Common__GenericMarshalling_i
+import opened Common__NodeIdentity_i
+import opened Common__NetClient_i
+import opened Common__Util_i
+import opened Raft__CBroadcast_i
+import opened Raft__CTypes_i
+import opened Raft__ConfigState_i
+import opened Raft__CMessage_i
+import opened Raft__PacketParsing_i
+import opened Logic__Option_i
+
+//////////////////////////////////////////////////////////////////////////////
+// These functions relate NetEvent to Raft's LIoOps.
+// 
+
+// NetEvent
+predicate NetEventIsAbstractable(evt:NetEvent)
+{
+  match evt
+    case LIoOpSend(s) => NetPacketIsAbstractable(s)
+    case LIoOpReceive(r) => NetPacketIsAbstractable(r)
+    case LIoOpTimeoutReceive => true
+    case LIoOpReadClock(t) => true
+}
+
+function AbstractifyNetEventToRaftIo(evt:NetEvent) : RaftIo
+  requires NetEventIsAbstractable(evt)
+{
+  match evt
+    case LIoOpSend(s) => LIoOpSend(AbstractifyNetPacketToRaftPacket(s))
+    case LIoOpReceive(r) => LIoOpReceive(AbstractifyNetPacketToRaftPacket(r))
+    case LIoOpTimeoutReceive => LIoOpTimeoutReceive()
+    case LIoOpReadClock(t) => LIoOpReadClock(t as int)
+}
+
+// NetEventLog
+predicate NetEventLogIsAbstractable(rawlog:seq<NetEvent>)
+{
+  forall i :: 0<=i<|rawlog| ==> NetEventIsAbstractable(rawlog[i])
+}
+
+function {:opaque} AbstractifyRawLogToIos(rawlog:seq<NetEvent>) : seq<RaftIo>
+  requires NetEventLogIsAbstractable(rawlog)
+  ensures |AbstractifyRawLogToIos(rawlog)| == |rawlog|
+  ensures forall i {:trigger AbstractifyNetEventToRaftIo(rawlog[i])} {:trigger AbstractifyRawLogToIos(rawlog)[i]} :: 0<=i<|rawlog| ==> AbstractifyRawLogToIos(rawlog)[i] == AbstractifyNetEventToRaftIo(rawlog[i])
+{
+  if (rawlog==[]) then [] else [AbstractifyNetEventToRaftIo(rawlog[0])] + AbstractifyRawLogToIos(rawlog[1..])
+}
+
+predicate RawIoConsistentWithSpecIO(rawlog:seq<NetEvent>, ios:seq<RaftIo>)
+{
+  && NetEventLogIsAbstractable(rawlog)
+  && AbstractifyRawLogToIos(rawlog) == ios
+}
+
+predicate OnlySentMarshallableData(rawlog:seq<NetEvent>)
+{
+  forall io :: io in rawlog && io.LIoOpSend? ==> NetPacketBound(io.s.msg) && Marshallable(RaftDemarshallData(io.s.msg))
+}
+
+
+//////////////////////////////////////////////////////////////////////////////
+// These methods wrap the raw NetClient interface
+//
+
+datatype ReceiveResult = RRFail() | RRTimeout() | RRPacket(cpacket:CPacket)
+
+method{:timeLimitMultiplier 2} Receive(netClient:NetClient, localAddr:EndPoint, config:ConfigState, msg_grammar:G) returns (rr:ReceiveResult, ghost netEvent:NetEvent)
+  requires NetClientIsValid(netClient)
+  requires EndPoint(netClient.MyPublicKey()) == localAddr
+  //requires KnownSendersMatchConfig(config)
+  requires ConfigStateIsValid(config)
+  requires msg_grammar == CMessage_grammar()
+  modifies NetClientRepr(netClient)
+  ensures netClient.env == old(netClient.env)
+  ensures netClient.MyPublicKey() == old(netClient.MyPublicKey())
+  ensures NetClientOk(netClient) <==> !rr.RRFail?
+  ensures old(NetClientRepr(netClient)) == NetClientRepr(netClient)
+  ensures !rr.RRFail? ==>
+            && netClient.IsOpen()
+            && old(netClient.env.net.history()) + [netEvent] == netClient.env.net.history()
+  ensures rr.RRTimeout? ==> netEvent.LIoOpTimeoutReceive?;
+  ensures rr.RRPacket? ==>
+            && netEvent.LIoOpReceive?
+            && NetPacketIsAbstractable(netEvent.r)
+            && CPacketIsAbstractable(rr.cpacket)
+            && CMessageIs64Bit(rr.cpacket.msg)
+            && EndPointIsValidPublicKey(rr.cpacket.src)
+            && AbstractifyCPacketToRaftPacket(rr.cpacket) == AbstractifyNetPacketToRaftPacket(netEvent.r)
+            && rr.cpacket.msg == RaftDemarshallData(netEvent.r.msg)
+            && RaftEndPointIsValid(rr.cpacket.src, config)
+{
+  var timeout := 0;
+  ghost var old_net_history := netClient.env.net.history();
+  var ok, timedOut, remote, buffer := netClient.Receive(timeout);
+
+  if (!ok) {
+    rr := RRFail();
+    return;
+  }
+
+  if (timedOut) {
+    rr := RRTimeout();
+    netEvent := LIoOpTimeoutReceive(); 
+    return;
+  }
+
+  var srcEp:EndPoint := EndPoint(remote);
+  netEvent := LIoOpReceive(LPacket(EndPoint(netClient.MyPublicKey()), srcEp, buffer[..]));
+  assert netClient.env.net.history() == old_net_history + [netEvent];
+  lemma_CMessageGrammarValid();
+  var cmessage := RaftDemarshallDataMethod(buffer, msg_grammar);
+
+  var cpacket := CPacket(localAddr, srcEp, cmessage);
+  rr := RRPacket(cpacket);
+  assert netClient.env.net.history() == old_net_history + [netEvent];
+
+  assert EndPointIsValidPublicKey(EndPoint(netClient.MyPublicKey()));
+  assert RaftEndPointIsValid(rr.cpacket.src, config);
+  assert AbstractifyCPacketToRaftPacket(rr.cpacket) == AbstractifyNetPacketToRaftPacket(netEvent.r);
+}
+
+method ReadClock(netClient:NetClient) returns (clock:CClockReading, ghost clockEvent:NetEvent)
+  requires NetClientIsValid(netClient)
+  modifies NetClientRepr(netClient)
+  ensures old(NetClientRepr(netClient)) == NetClientRepr(netClient)
+  ensures NetClientIsValid(netClient)
+  ensures netClient.env == old(netClient.env)
+  ensures old(netClient.env.net.history()) + [clockEvent] == netClient.env.net.history()
+  ensures clockEvent.LIoOpReadClock?
+  ensures clock.t as int == clockEvent.t
+  ensures NetClientIsValid(netClient)
+  ensures NetEventIsAbstractable(clockEvent)
+  ensures netClient.MyPublicKey() == old(netClient.MyPublicKey())
+  // TODO we're going to call GetTime, which returns a single value.
+{
+  var t := Time.GetTime(netClient.env);
+  clockEvent := LIoOpReadClock(t as int);
+  clock := CClockReading(t);
+}
+
+predicate SendLogEntryReflectsPacket(event:NetEvent, cpacket:CPacket)
+{
+  && event.LIoOpSend?
+  && NetPacketIsAbstractable(event.s)
+  && CPacketIsAbstractable(cpacket)
+  && AbstractifyCPacketToRaftPacket(cpacket) == AbstractifyNetPacketToRaftPacket(event.s)
+}
+
+predicate SendLogReflectsPacket(netEventLog:seq<NetEvent>, packet:Option<CPacket>)
+{
+  match packet {
+    case Some(p) => |netEventLog| == 1 && SendLogEntryReflectsPacket(netEventLog[0], p)
+    case None => netEventLog == []
+  }
+}
+
+predicate SendLogReflectsPacketSeq(netEventLog:seq<NetEvent>, packets:seq<CPacket>)
+{
+  && |netEventLog| == |packets| 
+  && (forall i :: 0 <= i < |packets| ==> SendLogEntryReflectsPacket(netEventLog[i], packets[i]))
+}
+
+predicate SendLogMatchesRefinement(netEventLog:seq<NetEvent>, broadcast:CBroadcast, index:int)
+  requires CBroadcastIsAbstractable(broadcast)
+  requires broadcast.CBroadcast?
+  requires 0<=|netEventLog|<=|broadcast.dsts|
+  requires 0 <= index < |netEventLog|
+{
+  && netEventLog[index].LIoOpSend? && NetPacketIsAbstractable(netEventLog[index].s)
+  && AbstractifyCBroadcastToRaftPacketSeq(broadcast)[index] == AbstractifyNetPacketToRaftPacket(netEventLog[index].s)
+}
+
+predicate SendLogReflectsBroadcastPrefix(netEventLog:seq<NetEvent>, broadcast:CBroadcast)
+  requires CBroadcastIsAbstractable(broadcast)
+  requires broadcast.CBroadcast?
+{
+  && 0<=|netEventLog|<=|broadcast.dsts|
+  && forall i :: 0<=i<|netEventLog| ==> SendLogMatchesRefinement(netEventLog, broadcast, i)
+}
+
+predicate SendLogReflectsBroadcast(netEventLog:seq<NetEvent>, broadcast:CBroadcast)
+  requires CBroadcastIsAbstractable(broadcast)
+{
+  if broadcast.CBroadcastNop? then
+    netEventLog == []
+  else 
+    && SendLogReflectsBroadcastPrefix(netEventLog, broadcast)
+    && |netEventLog| == |broadcast.dsts|
+}
+
+lemma lemma_NetEventLogAppend(broadcast:CBroadcast, netEventLog:seq<NetEvent>, netEvent:NetEvent)
+  requires broadcast.CBroadcast?
+  requires CBroadcastIsValid(broadcast)
+  requires SendLogReflectsBroadcastPrefix(netEventLog, broadcast)
+  requires |netEventLog| < |broadcast.dsts|
+  requires netEvent.LIoOpSend?
+  requires NetPacketIsAbstractable(netEvent.s)
+  requires CMessageIsAbstractable(RaftDemarshallData(netEvent.s.msg))
+  requires netEvent.s.dst == broadcast.dsts[|netEventLog|]
+  requires netEvent.s.src == broadcast.src
+  requires BufferRefinementAgreesWithMessageRefinement(broadcast.msg, netEvent.s.msg)
+  ensures SendLogReflectsBroadcastPrefix(netEventLog + [netEvent], broadcast)
+{
+  var i := |netEventLog|;
+
+  calc {
+    AbstractifyCBroadcastToRaftPacketSeq(broadcast)[i];
+    BuildLBroadcast(AbstractifyEndPointToNodeIdentity(broadcast.src), 
+                    AbstractifyEndPointsToNodeIdentities(broadcast.dsts), 
+                    AbstractifyCMessageToRaftMessage(broadcast.msg))[i];
+    LPacket(AbstractifyEndPointsToNodeIdentities(broadcast.dsts)[i], 
+            AbstractifyEndPointToNodeIdentity(broadcast.src), 
+            AbstractifyCMessageToRaftMessage(broadcast.msg));
+    LPacket(AbstractifyEndPointToNodeIdentity(netEvent.s.dst),
+            AbstractifyEndPointToNodeIdentity(netEvent.s.src),
+            AbstractifyCMessageToRaftMessage(RaftDemarshallData(netEvent.s.msg)));
+    AbstractifyNetPacketToRaftPacket(netEvent.s);
+  }
+
+  var new_log := netEventLog + [netEvent];
+
+  forall i' | 0 <= i' < |new_log|
+    ensures SendLogMatchesRefinement(new_log, broadcast, i')
+  {
+    if i' < |netEventLog| {
+      assert new_log[i'] == netEventLog[i'];
+      assert SendLogMatchesRefinement(netEventLog, broadcast, i');
+      assert SendLogMatchesRefinement(new_log, broadcast, i');
+    } else {
+      assert new_log[i'] == netEvent;
+      assert SendLogMatchesRefinement(new_log, broadcast, i');
+    }
+  }
+
+  calc ==> {
+    true;
+    forall i' :: 0 <= i' < |new_log| ==> SendLogMatchesRefinement(new_log, broadcast, i');
+    SendLogReflectsBroadcastPrefix(new_log, broadcast);
+    SendLogReflectsBroadcastPrefix(netEventLog + [netEvent], broadcast);
+  }
+}
+
+method SendBroadcast(netClient:NetClient, broadcast:CBroadcast, ghost localAddr_:EndPoint) returns (ok:bool, ghost netEventLog:seq<NetEvent>)
+  requires NetClientIsValid(netClient)
+  requires CBroadcastIsValid(broadcast)
+  requires EndPoint(netClient.MyPublicKey()) == localAddr_
+  requires broadcast.CBroadcast? ==> broadcast.src == localAddr_
+  modifies NetClientRepr(netClient)
+  ensures old(NetClientRepr(netClient)) == NetClientRepr(netClient)
+  ensures netClient.env == old(netClient.env)
+  ensures netClient.MyPublicKey() == old(netClient.MyPublicKey())
+  ensures NetClientOk(netClient) <==> ok
+  ensures ok ==>
+            && NetClientIsValid(netClient)
+            && netClient.IsOpen()
+            && old(netClient.env.net.history()) + netEventLog == netClient.env.net.history()
+            && OnlySentMarshallableData(netEventLog)
+            && SendLogReflectsBroadcast(netEventLog, broadcast)
+{
+  ok := true;
+  netEventLog := [];
+
+  if broadcast.CBroadcastNop? {
+    // No work to do!
+  } else {
+    // Do the marshalling work once
+    assert CMessageIsAbstractable(broadcast.msg);
+    assert Marshallable(broadcast.msg);
+    //var marshall_start_time := Time.GetDebugTimeTicks();
+    var buffer := RaftMarshall(broadcast.msg);
+    //var marshall_end_time := Time.GetDebugTimeTicks();
+    //RecordTimingSeq("SendBroadcast_PaxosMarshall", marshall_start_time, marshall_end_time);
+    assert NetPacketBound(buffer[..]);
+
+    calc ==> {
+      true;
+      CBroadcastIsValid(broadcast);
+      CBroadcastIsAbstractable(broadcast);
+      CMessageIsAbstractable(broadcast.msg);
+    }
+
+    var i:uint64 := 0;
+    while i < |broadcast.dsts| as uint64
+      invariant 0 <= i as int <= |broadcast.dsts|
+      invariant |netEventLog| == i as int
+      invariant NetClientRepr(netClient) == old(NetClientRepr(netClient))
+      invariant netClient.env == old(netClient.env)
+      invariant netClient.MyPublicKey() == old(netClient.MyPublicKey())
+      invariant NetClientIsValid(netClient)
+      invariant NetClientOk(netClient)
+      invariant old(netClient.env.net.history()) + netEventLog == netClient.env.net.history()
+      invariant NetPacketBound(buffer[..])
+      invariant Marshallable(RaftDemarshallData(buffer[..]))
+      invariant BufferRefinementAgreesWithMessageRefinement(broadcast.msg, buffer[..])
+      invariant SendLogReflectsBroadcastPrefix(netEventLog, broadcast)
+      invariant CMessageIsAbstractable(RaftDemarshallData(buffer[..]))
+      invariant OnlySentMarshallableData(netEventLog)
+    {
+      ghost var netEventLog_old := netEventLog;
+
+      // Construct the remote address -- TODO: Only do this once per replica!
+      var dstEp:EndPoint := broadcast.dsts[i];
+
+      ok := netClient.Send(dstEp.public_key, buffer);
+      if (!ok) { return; }
+
+      ghost var netEvent := LIoOpSend(LPacket(dstEp, EndPoint(netClient.MyPublicKey()), buffer[..]));
+      netEventLog := netEventLog + [netEvent];
+
+      lemma_NetEventLogAppend(broadcast, netEventLog_old, netEvent);
+
+      i := i + 1;
+    }
+  }
+}
+
+method SendPacket(netClient:NetClient, packets:OutboundPackets, ghost localAddr_:EndPoint) returns (ok:bool, ghost netEventLog:seq<NetEvent>)
+  requires NetClientIsValid(netClient)
+  requires packets.OutboundPacket?
+  requires OutboundPacketsIsValid(packets)
+  requires EndPoint(netClient.MyPublicKey()) == localAddr_
+  requires OutboundPacketsHasCorrectSrc(packets, localAddr_)
+  modifies NetClientRepr(netClient)
+  ensures old(NetClientRepr(netClient)) == NetClientRepr(netClient)
+  ensures netClient.env == old(netClient.env)
+  ensures netClient.MyPublicKey() == old(netClient.MyPublicKey())
+  ensures NetClientOk(netClient) <==> ok
+  ensures ok ==> && NetClientIsValid(netClient)
+                 && netClient.IsOpen()
+                 && old(netClient.env.net.history()) + netEventLog == netClient.env.net.history()
+                 && OnlySentMarshallableData(netEventLog)
+                 && SendLogReflectsPacket(netEventLog, packets.p)
+{
+  var j:uint64 := 0;
+  netEventLog := [];
+  ok := true;
+  var opt_packet := packets.p;
+
+  if opt_packet.None? {
+
+  } else {
+    var cpacket := opt_packet.v;
+
+    ghost var netEventLog_old := netEventLog;
+
+    // Construct the remote address
+    var dstEp:EndPoint := cpacket.dst;
+
+    assert CMessageIsAbstractable(cpacket.msg);
+    assert Marshallable(cpacket.msg);
+    var marshall_start_time := Time.GetDebugTimeTicks();
+    var buffer := RaftMarshall(cpacket.msg);
+    var marshall_end_time := Time.GetDebugTimeTicks();
+    RecordTimingSeq("SendBatch_PaxosMarshall", marshall_start_time, marshall_end_time);
+
+    ghost var data := buffer[..];
+    assert BufferRefinementAgreesWithMessageRefinement(cpacket.msg, data);
+
+    ok := netClient.Send(dstEp.public_key, buffer);
+    if (!ok) { return; }
+
+    ghost var netEvent := LIoOpSend(LPacket(dstEp, EndPoint(netClient.MyPublicKey()), buffer[..]));
+    ghost var net := netEvent.s;
+
+    calc {
+      AbstractifyCPacketToRaftPacket(cpacket);
+      LPacket(AbstractifyEndPointToNodeIdentity(cpacket.dst), AbstractifyEndPointToNodeIdentity(cpacket.src), AbstractifyCMessageToRaftMessage(cpacket.msg));
+      LPacket(AbstractifyEndPointToNodeIdentity(net.dst), AbstractifyEndPointToNodeIdentity(net.src), AbstractifyCMessageToRaftMessage(cpacket.msg));
+      AbstractifyBufferToRaftPacket(net.src, net.dst, data);
+      AbstractifyBufferToRaftPacket(net.src, net.dst, net.msg);
+      AbstractifyNetPacketToRaftPacket(netEvent.s);
+    }
+    assert SendLogEntryReflectsPacket(netEvent, cpacket);
+    netEventLog := [netEvent];
+  }
+}
+
+method{:timeLimitMultiplier 2} SendPacketSequence(netClient:NetClient, packets:OutboundPackets, ghost localAddr_:EndPoint) returns (ok:bool, ghost netEventLog:seq<NetEvent>)
+  requires NetClientIsValid(netClient)
+  requires OutboundPacketsIsValid(packets)
+  requires packets.PacketSequence?
+  requires EndPoint(netClient.MyPublicKey()) == localAddr_
+  requires OutboundPacketsHasCorrectSrc(packets, localAddr_)
+  modifies NetClientRepr(netClient)
+  ensures old(NetClientRepr(netClient)) == NetClientRepr(netClient)
+  ensures netClient.env == old(netClient.env)
+  ensures netClient.MyPublicKey() == old(netClient.MyPublicKey())
+  ensures NetClientOk(netClient) <==> ok
+  ensures ok ==>
+            && NetClientIsValid(netClient)
+            && netClient.IsOpen()
+            && old(netClient.env.net.history()) + netEventLog == netClient.env.net.history()
+            && OnlySentMarshallableData(netEventLog)
+            && SendLogReflectsPacketSeq(netEventLog, packets.s)
+{
+  var cpackets := packets.s;
+  var j:uint64 := 0;
+  netEventLog := [];
+  ok := true;
+    
+  ghost var netEventLog_old := netEventLog;
+  ghost var netClientEnvHistory_old := old(netClient.env.net.history());
+  var i:uint64 := 0;
+
+  while i < |cpackets| as uint64
+    invariant old(NetClientRepr(netClient)) == NetClientRepr(netClient)
+    invariant netClient.env == old(netClient.env)
+    invariant netClient.MyPublicKey() == old(netClient.MyPublicKey())
+    invariant NetClientOk(netClient) <==> ok
+    invariant ok ==> ( NetClientIsValid(netClient) && netClient.IsOpen())
+    invariant ok ==> netClientEnvHistory_old + netEventLog == netClient.env.net.history()
+    invariant (i == 0) ==> |netEventLog| == 0
+    invariant (0 < i as int < |cpackets|) ==> |netEventLog| == |cpackets[0..i]|
+    invariant (0 < i as int < |cpackets|) ==> SendLogReflectsPacketSeq(netEventLog, cpackets[0..i]);
+    invariant (i as int >= |cpackets|) ==> SendLogReflectsPacketSeq(netEventLog, cpackets);
+    invariant OnlySentMarshallableData(netEventLog)
+  {
+    var cpacket := cpackets[i];
+    // Construct the remote address
+    var dstEp:EndPoint := cpacket.dst;
+    assert cpacket in cpackets;
+    assert OutboundPacketsIsValid(packets);
+
+    assert CMessageIsAbstractable(cpacket.msg);
+         
+    assert Marshallable(cpacket.msg);
+    var buffer := RaftMarshall(cpacket.msg);
+
+    ghost var data := buffer[..];
+    assert BufferRefinementAgreesWithMessageRefinement(cpacket.msg, data);
+
+    ok := netClient.Send(dstEp.public_key, buffer);
+    if (!ok) { return; }
+
+    ghost var netEvent := LIoOpSend(LPacket(dstEp, EndPoint(netClient.MyPublicKey()), buffer[..]));
+    ghost var net := netEvent.s;
+
+    calc {
+      AbstractifyCPacketToRaftPacket(cpacket);
+      LPacket(AbstractifyEndPointToNodeIdentity(cpacket.dst), AbstractifyEndPointToNodeIdentity(cpacket.src), AbstractifyCMessageToRaftMessage(cpacket.msg));
+      LPacket(AbstractifyEndPointToNodeIdentity(net.dst), AbstractifyEndPointToNodeIdentity(net.src), AbstractifyCMessageToRaftMessage(cpacket.msg));
+      AbstractifyBufferToRaftPacket(net.src, net.dst, data);
+      AbstractifyBufferToRaftPacket(net.src, net.dst, net.msg);
+      AbstractifyNetPacketToRaftPacket(netEvent.s);
+    }
+        
+    assert SendLogEntryReflectsPacket(netEvent, cpacket);
+        
+    netEventLog := netEventLog + [netEvent];
+    assert cpackets[0..(i as int+1)] == cpackets[0..i as int] + [cpacket];
+    assert SendLogReflectsPacketSeq(netEventLog, cpackets[0..(i as int+1)]);
+    i := i + 1;
+  }
+}
+
+
+}
