ironfleet/src/Dafny/Distributed/Impl/Raft/QRelations.i.dfy
@@ -1,0 +1,55 @@
+include "../../Protocol/Raft/Server.i.dfy"
+include "../../Protocol/Raft/ServerScheduler.i.dfy"
+include "../../Protocol/Raft/Types.i.dfy"
+
+module Raft__QRelations_i {
+
+import opened Raft__Types_i
+import opened Raft__Server_i
+import opened Raft__ServerScheduler_i
+
+
+predicate {:opaque} Q_RaftServer_Next_ProcessPacket(server:RaftServer, server':RaftServer, ios:seq<RaftIo>)
+{
+  RaftServerNextProcessPacket(server, server', ios)
+}
+
+predicate {:opaque} Q_RaftScheduler_Next(sched:RaftServerScheduler, sched':RaftServerScheduler, ios:seq<RaftIo>)
+{
+  RaftServerSchedulerNext(sched, sched', ios)
+}
+
+predicate {:opaque} Q_RaftServer_NoReceive_Next(server:RaftServer, nextActionIndex:int, server':RaftServer, ios:seq<RaftIo>)
+{
+  RaftServerNoReceiveNext(server, nextActionIndex, server', ios)
+}
+
+lemma lemma_EstablishQLSchedulerNext(server:RaftServer, server':RaftServer, ios:seq<RaftIo>, sched:RaftServerScheduler, sched':RaftServerScheduler)
+  requires 0 <= sched.nextActionIndex < RaftServerNumActions()
+  requires sched.nextActionIndex == 0 ==> Q_RaftServer_Next_ProcessPacket(server, server', ios)
+  requires sched.nextActionIndex == 1 ==> Q_RaftServer_NoReceive_Next(server, sched.nextActionIndex, server', ios)
+  requires sched.server == server
+  requires sched'.server == server'
+  requires sched'.nextActionIndex == (sched.nextActionIndex+1)%RaftServerNumActions()
+  ensures Q_RaftScheduler_Next(sched, sched', ios)
+{
+  reveal Q_RaftServer_Next_ProcessPacket();
+  reveal Q_RaftServer_NoReceive_Next();
+  reveal Q_RaftScheduler_Next();
+}
+
+lemma lemma_EstablishQRaftServerNextProcessPacketFromTimeout(server:RaftServer, server':RaftServer, ios:seq<RaftIo>)
+  requires |ios|==1
+  requires ios[0].LIoOpTimeoutReceive?
+  requires server==server'
+  ensures Q_RaftServer_Next_ProcessPacket(server, server', ios)
+{
+  reveal Q_RaftServer_Next_ProcessPacket();
+}
+
+predicate {:opaque} Q_RaftServerScheduler_Next(s:RaftServerScheduler, s':RaftServerScheduler, ios:seq<RaftIo>)
+{
+  RaftServerSchedulerNext(s, s', ios)
+}
+
+}
