ironfleet/src/Dafny/Distributed/Impl/Raft/ServerImplMain.i.dfy
@@ -1,0 +1,214 @@
+include "../../Common/Framework/Environment.s.dfy"
+include "../../Common/Collections/Seqs.i.dfy"
+include "../../../Libraries/Math/mod_auto.i.dfy"
+include "../../Protocol/Raft/Server.i.dfy"
+include "../../Protocol/Raft/ServerScheduler.i.dfy"
+include "../../Protocol/Raft/Types.i.dfy"
+include "../Common/GenericMarshalling.i.dfy"
+// include "NetRSL.i.dfy"
+include "CTypes.i.dfy"
+include "PacketParsing.i.dfy"
+include "QRelations.i.dfy"
+include "ServerImpl.i.dfy"
+include "ServerImplProcessPacketX.i.dfy"
+
+module LiveRSL__ReplicaImplMain_i {
+
+import opened Environment_s
+import opened Native__Io_s
+import opened Native__NativeTypes_s
+import opened Collections__Seqs_i
+import opened Math__mod_auto_i
+import opened Raft__Server_i
+import opened Raft__ServerScheduler_i
+import opened Raft__Types_i
+import opened Common__GenericMarshalling_i
+import opened Common__NetClient_i
+import opened Raft__CTypes_i
+import opened Raft__PacketParsing_i
+import opened Raft__QRelations_i
+import opened Raft__ServerImpl_i
+import opened Raft__ServerImplProcessPacketX_i
+
+method {:timeLimitMultiplier 2} rollActionIndex(a:uint64) returns (a':uint64)
+  requires 0 <= a as int < 2
+  ensures a' as int == ((a as int) + 1) % RaftServerNumActions()
+{
+  lemma_mod_auto(2);
+  if (a >= 1) {
+    a' := 0;
+  } else {
+    a' := (a + 1);
+  }
+}
+
+predicate IosReflectIgnoringUnsendable(ios:seq<LIoOp<EndPoint, seq<byte>>>)
+{
+  && |ios| == 1
+  && ios[0].LIoOpReceive?
+  && (|| !Demarshallable(ios[0].r.msg, CMessage_grammar())
+     || !Marshallable(parse_Message(DemarshallFunc(ios[0].r.msg, CMessage_grammar()))))
+}
+    
+predicate HostNextIgnoreUnsendable(s:RaftServerScheduler, s':RaftServerScheduler, ios:seq<LIoOp<EndPoint, seq<byte>>>)
+{
+  && s.nextActionIndex == 0
+  && s' == s.(nextActionIndex := 1)
+  && IosReflectIgnoringUnsendable(ios)
+}
+
+
+method {:timeLimitMultiplier 2} ServerNextMainProcessPacketX(server_impl:ServerImpl)
+  returns (ok:bool, ghost netEventLog:seq<NetEvent>, ghost ios:seq<RaftIo>)
+  requires server_impl.Valid()
+  requires server_impl.nextActionIndex == 0
+  modifies server_impl.repr
+  ensures server_impl.repr == old(server_impl.repr)
+  ensures server_impl.net_client != null
+  ensures server_impl.Env().Valid() && server_impl.Env().ok.ok() ==> ok
+  ensures server_impl.Env() == old(server_impl.Env());
+  ensures ok ==>
+            && server_impl.Valid()
+            && (|| Q_RaftScheduler_Next(old(server_impl.AbstractifyToRaftServerScheduler()), server_impl.AbstractifyToRaftServerScheduler(), ios)
+               || HostNextIgnoreUnsendable(old(server_impl.AbstractifyToRaftServerScheduler()), server_impl.AbstractifyToRaftServerScheduler(), netEventLog))
+            // && RawIoConsistentWithSpecIO(netEventLog, ios)
+            // && OnlySentMarshallableData(netEventLog)
+            && old(server_impl.Env().net.history()) + netEventLog == server_impl.Env().net.history()
+{
+  ghost var server_old := old(server_impl.AbstractifyToRaftServer());
+  ghost var scheduler_old := old(server_impl.AbstractifyToRaftServerScheduler());
+
+  assert scheduler_old.nextActionIndex == 0;
+
+  //print ("Replica_Next_main Enter\n");
+  assert scheduler_old.server == server_old;
+  ok, netEventLog, ios := Server_Next_ProcessPacketX(server_impl);
+  if (!ok) { return; }
+
+  assert server_impl.Valid();
+
+  // Mention unchanged predicates over mutable state in the old heap.
+  ghost var net_client_old := server_impl.net_client;
+  ghost var net_addr_old := server_impl.net_client.MyPublicKey();
+  assert NetClientIsValid(net_client_old);
+
+  ghost var server := server_impl.AbstractifyToRaftServer();
+  server_impl.nextActionIndex := 1;
+  ghost var scheduler := server_impl.AbstractifyToRaftServerScheduler();
+
+  // Mention unchanged predicates over mutable state in the new heap.
+  assert net_client_old == server_impl.net_client;
+  assert NetClientIsValid(server_impl.net_client);
+  assert net_addr_old == server_impl.net_client.MyPublicKey();
+
+  assert server_impl.Valid();
+
+  calc {
+    scheduler.nextActionIndex;
+    server_impl.nextActionIndex as int;
+    1;
+      { lemma_mod_auto(RaftServerNumActions()); }
+    (1)%RaftServerNumActions();
+    (scheduler_old.nextActionIndex+1)%RaftServerNumActions();
+  }
+
+  if Q_RaftServer_Next_ProcessPacket(old(server_impl.AbstractifyToRaftServer()), server_impl.AbstractifyToRaftServer(), ios) {
+    lemma_EstablishQLSchedulerNext(server_old, server, ios, scheduler_old, scheduler);
+    assert Q_RaftScheduler_Next(old(server_impl.AbstractifyToRaftServerScheduler()), server_impl.AbstractifyToRaftServerScheduler(), ios);
+  }
+  else {
+    assert IosReflectIgnoringUnsendable(netEventLog);
+    assert old(server_impl.AbstractifyToRaftServer()) == server_impl.AbstractifyToRaftServer();
+    assert HostNextIgnoreUnsendable(old(server_impl.AbstractifyToRaftServerScheduler()), server_impl.AbstractifyToRaftServerScheduler(), netEventLog);
+  }
+}
+
+method ServerNextMainReadClock(r:ServerImpl)
+  returns (ok:bool, ghost netEventLog:seq<NetEvent>, ghost ios:seq<RaftIo>)
+  requires r.Valid()
+  requires r.nextActionIndex == 1
+  modifies r.repr
+  ensures r.repr == old(r.repr)
+  ensures r.net_client != null
+  ensures r.Env().Valid() && r.Env().ok.ok() ==> ok
+  ensures r.Env() == old(r.Env());
+  ensures ok ==>
+            && r.Valid()
+            // TOPROVE
+            // && Q_RaftServerScheduler_Next(old(r.AbstractifyToRaftServerScheduler()), r.AbstractifyToRaftServerScheduler(), ios)
+            // && RawIoConsistentWithSpecIO(netEventLog, ios)
+            // && OnlySentMarshallableData(netEventLog)
+            && old(r.Env().net.history()) + netEventLog == r.Env().net.history()
+{
+  var curActionIndex := r.nextActionIndex;
+
+  ghost var server_old := old(r.AbstractifyToRaftServer());
+  ghost var scheduler_old := old(r.AbstractifyToRaftServerScheduler());
+
+  assert scheduler_old.server == server_old;
+  ok, netEventLog, ios := Server_Next_NoReceive_ReadClock(r);
+  if (!ok) { return; }
+
+  assert r.Valid();
+
+  // Mention unchanged predicates over mutable state in the old heap.
+  ghost var net_client_old := r.net_client;
+  ghost var net_addr_old := r.net_client.MyPublicKey();
+  assert NetClientIsValid(net_client_old);
+
+  ghost var replica := r.AbstractifyToRaftServer();
+  var nextActionIndex' := rollActionIndex(r.nextActionIndex);
+  r.nextActionIndex := nextActionIndex';
+  ghost var scheduler := r.AbstractifyToRaftServerScheduler();
+
+  // Mention unchanged predicates over mutable state in the new heap.
+  assert net_client_old == r.net_client;
+  assert NetClientIsValid(r.net_client);
+  assert net_addr_old == r.net_client.MyPublicKey();
+
+  assert r.Valid();
+        
+  calc {
+    scheduler.nextActionIndex;
+    r.nextActionIndex as int;
+    nextActionIndex' as int;
+    ((curActionIndex+1) as int)%RaftServerNumActions();
+    (scheduler_old.nextActionIndex+1)%RaftServerNumActions();
+  }
+
+  lemma_EstablishQLSchedulerNext(server_old, replica, ios, scheduler_old, scheduler);
+  assert Q_RaftServerScheduler_Next(old(r.AbstractifyToRaftServerScheduler()), r.AbstractifyToRaftServerScheduler(), ios);
+}
+
+
+method Server_Next_main(server_impl:ServerImpl)
+  returns (ok:bool, ghost net_event_log:seq<NetEvent>, ghost ios:seq<RaftIo>)
+  requires server_impl.Valid()
+  modifies server_impl.app_state, server_impl.repr
+  ensures server_impl.repr == old(server_impl.repr)
+  ensures server_impl.net_client != null
+  ensures server_impl.Env().Valid() && server_impl.Env().ok.ok() ==> ok
+  ensures server_impl.Env() == old(server_impl.Env());
+  ensures ok ==>
+            && server_impl.Valid()
+            // TOPROVE
+            && (|| Q_RaftScheduler_Next(old(server_impl.AbstractifyToRaftServerScheduler()), server_impl.AbstractifyToRaftServerScheduler(), ios)
+               || HostNextIgnoreUnsendable(old(server_impl.AbstractifyToRaftServerScheduler()), server_impl.AbstractifyToRaftServerScheduler(), net_event_log))
+            // && RawIoConsistentWithSpecIO(net_event_log, ios)
+            // && OnlySentMarshallableData(net_event_log)
+            && old(server_impl.Env().net.history()) + net_event_log == server_impl.Env().net.history()
+{
+  //print ("Replica_Next_main Enter\n");
+  if server_impl.nextActionIndex == 0 {
+    ok, net_event_log, ios := ServerNextMainProcessPacketX(server_impl);
+  }
+  else if (server_impl.nextActionIndex == 1) {
+    ok, net_event_log, ios := ServerNextMainReadClock(server_impl);
+  }
+  //print ("Replica_Next_main Exit\n");
+}
+
+
+
+
+}
