ironfleet/src/Dafny/Distributed/Impl/Raft/ServerImplNoReceiveClock.i.dfy
@@ -1,0 +1,85 @@
+include "../../Common/Collections/Seqs.i.dfy"
+include "../../../Libraries/Math/mod_auto.i.dfy"
+include "../../Protocol/Raft/Server.i.dfy"
+include "../../Protocol/Raft/Types.i.dfy"
+include "../Common/UpperBound.i.dfy"
+include "CBroadcast.i.dfy"
+include "CMessage.i.dfy"
+include "Config.i.dfy"
+include "CTypes.i.dfy"
+include "NetRaft.i.dfy"
+include "PacketParsing.i.dfy"
+include "QRelations.i.dfy"
+include "ServerImpl.i.dfy"
+// include "NetRSL.i.dfy"
+
+module Raft_ServerImplNoReceiveClock {
+
+import opened Native__Io_s
+import opened Native__NativeTypes_s
+import opened Collections__Seqs_i
+import opened Math__mod_auto_i
+import opened Common__NetClient_i
+import opened Common__UpperBound_i
+import opened Environment_s
+import opened Raft__CBroadcast_i
+import opened Raft__ConfigState_i
+import opened Raft__CTypes_i
+import opened Raft__CMessage_i
+import opened Raft__NetRaft_i
+import opened Raft__PacketParsing_i
+import opened Raft__QRelations_i
+import opened Raft__ServerImpl_i
+import opened Raft__Types_i
+
+method Server_Next_NoReceive_ReadClock(server_impl:ServerImpl)
+  returns (ok:bool, ghost net_event_log:seq<NetEvent>, ghost ios:seq<RaftIo>)
+  requires server_impl.nextActionIndex == 1
+  requires server_impl.Valid()
+  modifies server_impl.repr
+  // ensures server_impl.Repr == old(server_impl.Repr)
+  // ensures server_impl.netClient != null
+  // ensures ok == NetClientOk(server_impl.netClient)
+  // ensures server_impl.Env() == old(server_impl.Env())
+  // ensures ok ==>
+  //           && server_impl.Valid()
+  //           && server_impl.Env() == old(server_impl.Env())
+  //           && server_impl.nextActionIndex == old(server_impl.nextActionIndex)
+  //           && Q_LReplica_NoReceive_Next(old(server_impl.AbstractifyToLReplica()), server_impl.nextActionIndex as int, server_impl.AbstractifyToLReplica(), ios)
+  //           && OnlySentMarshallableData(netEventLog)
+  //           && RawIoConsistentWithSpecIO(netEventLog, ios)
+  //           && old(server_impl.Env().net.history()) + netEventLog == server_impl.Env().net.history()
+{
+  ok := true;
+  net_event_log := [];
+  ios := [];
+
+  if server_impl.nextActionIndex == 1 {
+    var clock,netEvent0 := ReadClock(server_impl.net_client);
+    ghost var io0 := LIoOpReadClock(clock.t as int);
+
+    if (server_impl.role.Leader?) {
+      ok := true;
+      if (clock.t >= server_impl.next_heartbeat_time) {
+        var const_params := server_impl.config.global_config.params;
+        var next_heartbeat_time := UpperBoundedAdditionImpl(clock.t, const_params.heartbeat_timeout, const_params.max_integer_value);
+        server_impl.next_heartbeat_time := next_heartbeat_time;
+        var msg := CMessage_AppendEntries(server_impl.current_term, server_impl.config.server_ep, 0, 0, [], 0);
+        var packets := BuildBroadcastToEveryone(server_impl.config.global_config, server_impl.config.server_ep, msg);
+        var packets_sent := Broadcast(packets);
+        ghost var log_tail, ios_tail;
+        ok, log_tail, ios_tail := DeliverOutboundPackets(server_impl, packets_sent);
+        if (!ok) { return; }
+        ghost var ios_head := [io0];
+        ghost var log_head := [netEvent0];
+        ios := ios_head + ios_tail;
+        net_event_log := log_head + log_tail;
+
+      } else {
+        replica', packets_sent := ReplicaNextReadClockMaybeSendHeartbeatSkip(replica, clock);
+      }
+    }
+  }
+}
+
+}
