ironfleet/src/Dafny/Distributed/Impl/Raft/ServerImplProcessPacketX.i.dfy
@@ -1,0 +1,89 @@
+include "../../Common/Collections/Seqs.i.dfy"
+include "../../../Libraries/Math/mod_auto.i.dfy"
+include "../../Protocol/Raft/Server.i.dfy"
+include "../../Protocol/Raft/Types.i.dfy"
+include "../Common/UpperBound.i.dfy"
+include "CMessage.i.dfy"
+include "Config.i.dfy"
+include "CTypes.i.dfy"
+include "NetRaft.i.dfy"
+include "PacketParsing.i.dfy"
+include "QRelations.i.dfy"
+include "ServerImpl.i.dfy"
+// include "NetRSL.i.dfy"
+
+module Raft__ServerImplProcessPacketX_i {
+
+import opened Native__Io_s
+import opened Native__NativeTypes_s
+import opened Collections__Seqs_i
+import opened Math__mod_auto_i
+import opened Common__NetClient_i
+import opened Common__UpperBound_i
+import opened Environment_s
+import opened Raft__ConfigState_i
+import opened Raft__CTypes_i
+import opened Raft__CMessage_i
+import opened Raft__NetRaft_i
+import opened Raft__PacketParsing_i
+import opened Raft__QRelations_i
+import opened Raft__ServerImpl_i
+import opened Raft__Types_i
+
+method Server_Next_ProcessPacketX(server_impl:ServerImpl)
+  returns (ok:bool, ghost net_event_log:seq<NetEvent>, ghost ios:seq<RaftIo>)
+  requires server_impl.Valid()
+  requires ConfigStateIsValid(server_impl.config.global_config)
+  modifies server_impl, server_impl.repr, server_impl.net_client;
+  // ensures server_impl.repr == old(server_impl.repr)
+  // ensures server_impl.net_client != null
+  // ensures ok == NetClientOk(server_impl.net_client)
+  // ensures server_impl.Env().Valid() && server_impl.Env().ok.ok() ==> ok
+  // ensures server_impl.Env() == old(server_impl.Env());
+  // ensures ok ==> 
+  //           && server_impl.Valid()
+  //           && server_impl.nextActionIndex == old(server_impl.nextActionIndex)
+  //           && (|| Q_RaftServer_Next_ProcessPacket(old(server_impl.AbstractifyToRaftServer()), server_impl.AbstractifyToRaftServer(), ios)
+  //               || (&& IosReflectIgnoringUnsendable(net_event_log)
+  //                  && old(server_impl.AbstractifyToRaftServer()) == server_impl.AbstractifyToRaftServer()))
+  //           && RawIoConsistentWithSpecIO(net_event_log, ios)
+  //           && OnlySentMarshallableData(net_event_log)
+  //           && old(server_impl.Env().net.history()) + net_event_log == server_impl.Env().net.history()
+{
+  ghost var old_net_history := server_impl.Env().net.history();
+
+  var rr, receive_event := Receive(server_impl.net_client, server_impl.config.server_ep, server_impl.config.global_config, server_impl.msg_grammar);
+  
+  if (rr.RRFail?) {
+    ok := false;
+    net_event_log := [];
+    ios := [];
+    return;
+  } else if (rr.RRTimeout?) {
+    ok := true;
+    net_event_log := [receive_event];
+    ios := [LIoOpTimeoutReceive()];
+  } else {
+    var marshallable := DetermineIfMessageMarshallable(rr.cpacket.msg);
+    if !marshallable {
+      ok := true;
+      ghost var receive_io := LIoOpReceive(AbstractifyNetPacketToRaftPacket(receive_event.r));
+      net_event_log := [receive_event];
+      ios := [receive_io];
+    } else if (rr.cpacket.msg.CMessage_AppendEntries?) {
+      ok := true;
+      var const_params := server_impl.config.global_config.params;
+      var clock, clock_event := ReadClock(server_impl.net_client);
+      var election_timeout_delta := GenerateElectionTimeout(const_params);
+      var next_election_time := UpperBoundedAdditionImpl(clock.t, election_timeout_delta, const_params.max_integer_value);
+      server_impl.next_election_time := next_election_time;
+    } else {
+      ok := true;
+      ghost var receive_io := LIoOpReceive(AbstractifyNetPacketToRaftPacket(receive_event.r));
+      net_event_log := [receive_event];
+      ios := [receive_io];
+    }
+  }
+}
+
+}
